Small edits

pset02_BinomialCoefficients/Pset2.v
@@ -83,6 +83,8 @@ Compute fact 4.
 Close Scope N_recursion_scope.
 Print fact.
 *)
+(*Close Scope N_recursion_scope.*)
+(*Print fact.*)
 
 (* Instead of writing "(fact x)" all the time, it's more convenient to just write "x!",
    so we make a Notation for this: *)
@@ -91,14 +93,18 @@ Local Notation "x !" := (fact x) (at level 12, format "x !").
 (* Exercise: Define a simple exponentiation function in the same style,
    so that "exp base n" equals "base^n". *)
 
-Definition exp(base: N): N -> N. Admitted.
+Definition exp(base: N): N -> N :=
+  recurse by cases
+  | 0 => 1
+  | n + 1 => base * recurse
+  end.
 
 (* Once you define "exp", you can replace "Admitted." below by "Proof. equality. Qed." *)
-Lemma test_exp_2_3: exp 2 3 = 8. Admitted.
-Lemma test_exp_3_2: exp 3 2 = 9. Admitted.
-Lemma test_exp_4_1: exp 4 1 = 4. Admitted.
-Lemma test_exp_5_0: exp 5 0 = 1. Admitted.
-Lemma test_exp_1_3: exp 1 3 = 1. Admitted.
+Lemma test_exp_2_3: exp 2 3 = 8. Proof. equality. Qed.
+Lemma test_exp_3_2: exp 3 2 = 9. Proof. equality. Qed.
+Lemma test_exp_4_1: exp 4 1 = 4. Proof. equality. Qed.
+Lemma test_exp_5_0: exp 5 0 = 1. Proof. equality. Qed.
+Lemma test_exp_1_3: exp 1 3 = 1. Proof. equality. Qed.
 
 (* Here's another recursive function defined in the same style to apply a function f to
    a range of values:
